{
  "nbformat": 4,
  "nbformat_minor": 0,
  "metadata": {
    "colab": {
      "provenance": [],
      "authorship_tag": "ABX9TyNgfTKwlI8bgW5zSWnkjgyG"
    },
    "kernelspec": {
      "name": "python3",
      "display_name": "Python 3"
    },
    "language_info": {
      "name": "python"
    }
  },
  "cells": [
    {
      "cell_type": "markdown",
      "source": [
        "### Chapman Kolmogorov relation:\n",
        "\n",
        "A time series of random variables is a Markov chain if\n",
        "\n",
        "$$\\Pr(X_t=x_t \\mid X_0=x_0, X_1=x_1,\\dots, X_{t-1}=x_{t-1})=\\Pr(X_t=x_t\\mid X_{t-1}=x_{t-1})$$\n",
        "\n",
        "They can be expressed as a transition probability matrix:\n",
        "\n",
        "$$\\begin{bmatrix}\n",
        "\\color{red}{\\text{initial}} &&\\color{blue}{\\text{state system moves to during the step}}&&&\\\\\n",
        "\\color{red}{\\text{state}}&&\\vdots&&&&\\\\\n",
        "\\color{red}{\\text{the}}&\\quad b&\\to\\to\\to\\to \\to\\to &d&&&&\\\\\n",
        "\\color{red}{\\text{matrix}}&&\\vdots&&\\\\\n",
        "\\color{red}{\\text{is in.}}&&\\vdots&\n",
        "\\end{bmatrix}$$\n",
        "\n",
        "So by choosing row $b$ and column $d$ we get the $\\Pr(d \\mid b).$ But what about making predictions several steps into the future? It amounts to powers of the transition probability matrix. The $n+m$ step transition probability matrix\n",
        "\n",
        "$$\\bf A^{n+m}=A^nA^m$$\n",
        "\n",
        "This is the Chapman Kolmogorov relation."
      ],
      "metadata": {
        "id": "U42rblVrQ8W1"
      }
    },
    {
      "cell_type": "markdown",
      "source": [
        "### Continuous time Markov Chains:\n",
        "\n",
        "The probability transition matrix is written as a function of time. And as such the following limit makes sense to ask:\n",
        "\n",
        "$$\\frac{\\rm d}{\\rm dt}P(t)=\\lim_{\\delta t\\to 0}\\frac{P(t+\\delta t) - P(t)}{\\delta t}$$\n",
        "\n",
        "where the $P(\\cdot)$ entries are transition matrices. This is called the Kolmogorov forward relation. Applying the Chapman-Kolmogorov relation:\n",
        "\n",
        "$$\\begin{align}\\frac{\\rm d}{\\rm dt}P(t)&=\\lim_{\\delta t\\to 0}\\frac{P(t+\\delta t) - P(t)}{\\delta t}\\\\\n",
        "&=\\lim_{\\delta t\\to 0}\\frac{P(t)P(\\delta t) - P(t)}{\\delta t}\\\\\n",
        "&=P(t)\\lim_{\\delta t\\to 0}\\frac{P(\\delta t) - I}{\\delta t}\\\\\n",
        "&=P(t)Q\n",
        "\\end{align}$$\n",
        "\n",
        "since all the rows in $P(\\delta t)$ should add up to $1$ as a transition probability matrix, subtracting the identity matrix $I$ implies that all rows of $Q$ must add up to $0.$ The matrix $Q$ is the **jump rate or generator matrix**.\n",
        "\n",
        "The solution is\n",
        "\n",
        "$$P(t)=e^{Qt}$$\n",
        "\n",
        "and\n",
        "\n",
        "$$e^{Qt}=I+ Qt+\\frac 1 2 Q^2 t^2+\\frac{1}{3!}Q^3t^3+\\cdots$$\n",
        "\n",
        "A steady state is reached when the transition probability vector is\n",
        "\n",
        "$$\\pi Q=0,$$\n",
        "\n",
        "inidcating that the change in $P(t)$ is $\\pi Q=0.$\n",
        "\n"
      ],
      "metadata": {
        "id": "XsenYCCWM5Vc"
      }
    },
    {
      "cell_type": "markdown",
      "source": [
        "### Poisson process:\n",
        "\n",
        "From [here](https://qr.ae/pGQpIt):\n",
        "\n",
        "> A Poisson process is one where the time between successive occurrences of an event follows an exponential distribution (the time you have to wait for the next occurrence of the event is independent of the time you have waited for so far).\n",
        ">\n",
        "> If the time is divided into equal intervals then the number of occurrences of an event in each time interval follows a Poisson distribution.\n",
        "\n",
        "The Poisson process is a continuous time Markov chain.\n",
        "\n",
        "If we choose a sufficiently small increment of time $\\delta t$ either $1$ event or $0$ events will have occurred. If the events occur with some mean rate of $\\lambda,$ on average $\\Pr(\\text{1 event})=\\lambda\\delta,$ and $\\Pr(\\text{0 events})=1 - \\lambda\\delta.$ The mean gap in time is $1/\\lambda.$\n",
        "\n",
        "To find $\\Pr(n,t)$ we look at the $\\Pr(n, t+\\delta t).$ This leaves two possibilities: Either all $n$ occurrences happened before $t,$ with probability $\\Pr(n,t)\\left(1-\\lambda \\delta t\\right).$ Or $n-1$ events occurred before $t$ and $1$ event between $t$ and $t+\\delta.$ This latter scenario has probability $\\Pr(n-1,t)\\lambda \\delta t.$ Hence,\n",
        "\n",
        "$$\\Pr(n, t+\\delta t)=\\Pr(n-1,t)\\lambda \\delta t+\\Pr(n,t)\\left(1-\\lambda \\delta t\\right)$$\n",
        "\n",
        "It follows that\n",
        "\n",
        "$$\\frac{\\rm d}{\\rm dt}P(n,t)=\\lambda\\left(\\Pr(n-1,t)-\\Pr(n,t) \\right)$$\n",
        "\n",
        "with initial condition $\\Pr(n,0)=\\delta_{n,0},$ i.e. no events have occurred at time zero.\n",
        "\n",
        "The $\\Pr(0,t+\\delta t)=\\Pr(0,t)+\\left(1-\\lambda \\delta t \\right).$ This implies that\n",
        "\n",
        "$$\\frac{\\rm d \\Pr(0,t)}{\\rm dt}=-\\lambda \\Pr(0,t).$$\n",
        "\n",
        "Hence the probability of nothing happening decreases with time.\n",
        "\n",
        "We pay attention to the count of events across time:\n",
        "\n",
        "![](https://user-images.githubusercontent.com/9312897/154624693-189ebaf1-35a6-40c3-82a1-4a4750702363.png)\n",
        "\n",
        "The jump rate matrix is\n",
        "\n",
        "$$Q=\\lim_{\\delta t\\to 0}\\frac{P(\\delta t) - I}{\\delta t}=\\begin{bmatrix}-\\lambda& \\lambda & & &\\\\&-\\lambda &\\lambda &&\\\\&&-\\lambda&\\lambda \\\\&&&&\\ddots\\end{bmatrix}$$\n",
        "\n",
        "Why?\n",
        "\n",
        "$$\\small\\begin{bmatrix}\\frac{\\rm d P_{00}(t)}{\\rm dt}& \\frac{\\rm d P_{01}(t)}{\\rm dt} & \\frac{\\rm d P_{02}(t)}{\\rm dt} \\\\\\frac{\\rm d P_{10}(t)}{\\rm dt}&\\frac{\\rm d P_{11}(t)}{\\rm dt} &\\frac{\\rm d P_{12}(t)}{\\rm dt}\\\\\\frac{\\rm d P_{20}(t)}{\\rm dt}&\\frac{\\rm d P_{21}(t)}{\\rm dt}&\\frac{\\rm d P_{22}(t)}{\\rm dt} \\\\&&&&\\ddots\\end{bmatrix}\n",
        "=\\begin{bmatrix}P_{00}(t)& P_{01}(t) &P_{02}(t) \\\\P_{10}(t) &P_{11}(t) &P_{12}(t)\\\\P_{20}(t)&P_{21}(t)&P_{22}(t) \\\\&&&\\ddots\\end{bmatrix}\n",
        "\\begin{bmatrix}-\\lambda& \\lambda & & &\\\\&-\\lambda &\\lambda &&\\\\&&-\\lambda&\\lambda \\\\&&&&\\ddots\\end{bmatrix}$$\n",
        "\n",
        "So\n",
        "\n",
        "$$\\frac{\\rm d P_{00}(t)}{\\rm dt}=-\\lambda P_{00}(t)\\tag 1$$\n",
        "\n",
        "and\n",
        "\n",
        "$$\\frac{\\rm d P_{01}(t)}{\\rm dt}=\\lambda P_{00}(t) - \\lambda P_{01}(t)$$\n",
        "\n",
        "or in general,\n",
        "\n",
        "$$\\frac{\\rm d P_{0k}(t)}{\\rm dt}=\\lambda P_{0(k-1)}(t) - \\lambda P_{0k}(t)\\tag 2$$\n",
        "\n",
        "For $(1),$ since no events have occurred at the start ($0$ boundary condition - so P_{00}(0)=1):\n",
        "\n",
        "$$\\begin{align}\\int_1^{P_{00}(t)}\\frac{\\rm d P_{00}(t)}{P_{00}(t)}&=-\\int_0^t \\lambda \\rm dt\\\\[2 ex]\n",
        "\\log\\left(P_{00}(t) \\right)\\vert_1^{P_{00}(t)} &= -\\lambda t \\vert_0^t\\\\[2 ex]\n",
        "\\log\\left(P_{00}(t) \\right) - \\log(1) &= -\\lambda t\\\\[2 ex]\n",
        "P_{00}(t) = \\rm e^{-\\lambda t}\n",
        "\\end{align}$$\n",
        "\n",
        "This means that the probability that no events have happened by time $t$ decreases exponentially.\n",
        "\n",
        "For $(2),$ adding a factor of $P_{01}(t)$ to both sides, and using the integrating factor $\\rm e^{\\lambda t}$ (to be able to use the product rule, and plugging in $P_{00}(t)$ from the immediate prior result we can derive the following. Again, we assume that no events have happened at $t=0$ to set up the limits of integration (the probability that $1$ event had happened at $t=0$ is $0$):\n",
        "\n",
        "$$\\begin{align}\n",
        "\\frac{\\rm d P_{01}(t)}{\\rm dt}&=\\lambda P_{00}(t) - \\lambda P_{01}(t)\\\\[2 ex]\n",
        "\\frac{\\rm d P_{01}(t)}{\\rm dt}+ \\lambda P_{01}(t)&=\\lambda P_{00}(t) \\\\[2 ex]\n",
        "\\rm e^{\\lambda t} \\frac{\\rm d P_{01}(t)}{\\rm dt}+ \\rm e^{\\lambda t}\\lambda P_{01}(t)&=\\rm e^{\\lambda t}\\lambda P_{00}(t)\\\\[2 ex]\n",
        "\\rm e^{\\lambda t} \\frac{\\rm d P_{01}(t)}{\\rm dt}+ \\rm e^{\\lambda t}\\lambda P_{01}(t)&=\\rm e^{\\lambda t}\\lambda \\rm e^{-\\lambda t}\\\\[2ex]\n",
        "\\rm e^{\\lambda t} \\frac{\\rm d P_{01}(t)}{\\rm dt}+ \\rm e^{\\lambda t}\\lambda P_{01}(t)&=\\lambda \\\\[2ex]\n",
        " \\frac{\\rm d \\left( \\rm e^{\\lambda t}P_{01}(t)\\right)}{\\rm dt}&=\\lambda\\\\[2ex]\n",
        "\\int_0^{\\rm e^{\\lambda t}P_{01}(t)}\\rm d \\left( \\rm e^{\\lambda t}P_{01}(t)\\right)&=\\int_0^t \\lambda \\rm dt \\\\[2ex]\n",
        "\\rm e^{\\lambda t}P_{01}(t)&=\\lambda t\\\\[2ex]\n",
        "P_{01}(t)&=\\lambda t \\rm e^{-\\lambda t}\n",
        "\\end{align}$$\n",
        "\n",
        "Now we can use this result to plug into the derivation of $P_{02}(t)$ to get\n",
        "\n",
        "$$P_{02}(t)=\\frac{\\lambda^2 t^2}{2}\\rm e^{-\\lambda t}$$\n",
        "\n",
        "Looking at the pattern of the above results:\n",
        "\n",
        "$$P_{0n}(t)=\\frac{(\\lambda t)^n}{n!}\\rm e^{-\\lambda t}$$\n",
        "\n",
        "which is the Poisson PMF turned into a continuous expression."
      ],
      "metadata": {
        "id": "XwY9eVK3e3T_"
      }
    },
    {
      "cell_type": "markdown",
      "source": [
        "### Birth-Death Queues:\n",
        "\n",
        "![](https://user-images.githubusercontent.com/9312897/154734243-855942aa-4b36-4068-bbee-cb3ec3730291.png)\n",
        "\n",
        "Different from the counting process of events in a Poisson process, in this example of continuous time Markov chain there is a possibility of going back in counts. Each count is called a \"state.\" The \"birth\" occurs at times distributed exponentially with rate $\\lambda$. The departure or \"death\" occurs exponentially with parameter $\\mu.$\n",
        "\n",
        "The generating matrix is:\n",
        "\n",
        "$$Q=\\lim_{\\delta t\\to 0}\\frac{P(\\delta t) - I}{\\delta t}=\\begin{bmatrix}-\\lambda& \\lambda & & &\\\\\\mu&-(\\lambda+\\mu) &\\lambda &&\\\\&\\mu&-(\\lambda+\\mu)&\\lambda \\\\&&&&\\ddots\\end{bmatrix}$$\n"
      ],
      "metadata": {
        "id": "uKCwvf23QPaf"
      }
    }
  ]
}